DistributedSystems/VerifiedDS/src/Dafny/Distributed/Protocol/CausalMesh/proof/cache_does_not_decrease.dfy
@@ -1,0 +1,212 @@
+include "../distributed_system.dfy"
+// include "causalcut.dfy"
+include "packet_sending.dfy"
+include "properties.dfy"
+include "environment.dfy"
+// include "deps_are_met.dfy"
+// include "monotonic_read.dfy"
+include "../../../Common/Collections/Seqs.s.dfy"
+
+module CausalMesh_Proof_CacheDoesNotDecrease_i {
+import opened CausalMesh_Cache_i
+import opened CausalMesh_Message_i
+import opened CausalMesh_Types_i
+import opened Environment_s
+import opened CausalMesh_DistributedSystem_i
+import opened CausalMesh_Properties_i
+import opened CausalMesh_PullDeps_i
+import opened CausalMesh_Proof_Actions_i
+import opened Temporal__Temporal_s
+import opened CausalMesh_proof_Assumptions_i
+import opened CausalMesh_Proof_Constants_i
+import opened CausalMesh_Proof_PacketSending_i
+import opened CausalMesh_Proof_Properties_i
+// import opened CausalMesh_Proof_DepsAreMet_i
+// import opened CausalMesh_Proof_Monotonic_Read_i
+import opened CausalMesh_Proof_Environment_i
+import opened Collections__Seqs_s
+import opened Collections__Maps_i
+import opened Collections__Maps2_s
+
+lemma lemma_CMNextCacheDoesNotDecreasePrefix(
+    b:Behavior<CMState>,
+    i:int
+)
+    requires 0 <= i 
+    requires IsValidBehaviorPrefix(b, i+1)
+    requires forall j :: 0 <= j <= i ==> CMNext(b[j], b[j+1])
+    // requires AllServersAreCausalCut(b[0])
+    ensures forall j :: 0 <= j < i ==> ServerNextDoesNotDecreaseVersions(b[j], b[j+1])
+    decreases i
+{
+    if i == 0 {
+        return;
+    }
+
+    lemma_ConstantsAllConsistent(b, i-1);
+    lemma_ConstantsAllConsistent(b, i);
+
+    lemma_BehaviorValidImpliesOneStepValid(b, i);
+    assert CMNext(b[i-1], b[i]);
+
+    lemma_CMNextCacheDoesNotDecreasePrefix(b, i-1);
+    assert forall j :: 0 <= j < i - 1 ==> ServerNextDoesNotDecreaseVersions(b[j], b[j+1]);
+    lemma_CMNextCacheDoesNotDecrease(b, i-1);
+    assert ServerNextDoesNotDecreaseVersions(b[i-1], b[i]);
+    lemma_CMNextCacheDoesNotDecreasePrefix_helper(b, i);
+    assert forall j :: 0 <= j < i ==> ServerNextDoesNotDecreaseVersions(b[j], b[j+1]);
+}
+
+lemma lemma_CMNextCacheDoesNotDecreasePrefix_helper(
+    b:Behavior<CMState>,
+    i:int
+)
+    requires 0 <= i 
+    requires IsValidBehaviorPrefix(b, i)
+    requires forall j :: 0 <= j <= i ==> CMNext(b[j], b[j+1])
+    requires CMNext(b[i-1], b[i])
+    requires forall j :: 0 <= j < i - 1 ==> ServerNextDoesNotDecreaseVersions(b[j], b[j+1])
+    requires ServerNextDoesNotDecreaseVersions(b[i-1], b[i])
+    ensures forall j :: 0 <= j < i ==> ServerNextDoesNotDecreaseVersions(b[j], b[j+1])
+    decreases i
+{
+
+}
+
+lemma lemma_CMNextCacheDoesNotDecrease(b:Behavior<CMState>, i:int)
+    requires IsValidBehaviorPrefix(b, i+1)
+    requires 0 <= i
+    // requires forall j :: 0 <= j <= i ==> CMNext(b[j], b[j+1])
+    requires CMNext(b[i], b[i+1])
+    // requires ServerNextDoesNotDecreaseVersions(b[i-1], b[i])
+    ensures ServerNextDoesNotDecreaseVersions(b[i], b[i+1])
+{
+    var ps := b[i];
+    var ps' := b[i+1];
+
+    if ps.servers == ps'.servers {
+        assert ServerNextDoesNotDecreaseVersions(b[i], b[i+1]);
+    } 
+    else {
+        var idx :| 0 <= idx < |ps.servers| && ps.servers[idx] != ps'.servers[idx];
+        lemma_CMNextCacheDoesNotDecrease_helper(b, i, idx);
+    }
+}
+
+lemma lemma_CMNextCacheDoesNotDecrease_helper(b:Behavior<CMState>, i:int, idx:int)
+    requires IsValidBehaviorPrefix(b, i+1)
+    requires 0 <= i
+    requires 0 <= idx < |b[i].servers|
+    requires 0 <= idx < |b[i+1].servers|
+    requires b[i].servers[idx] != b[i+1].servers[idx]
+    // requires forall j :: 0 <= j < i ==> CMNext(b[j], b[j+1])
+    requires CMNext(b[i], b[i+1])
+    // requires ServerNextDoesNotDecreaseVersions(b[i-1], b[i])
+    ensures ServerNextDoesNotDecreaseVersions(b[i], b[i+1])
+{
+    var s := b[i].servers[idx].s;
+    var s' := b[i+1].servers[idx].s;
+
+    assert IsValidBehaviorPrefix(b, i+1);
+    assert 0 <= i;
+    assert 0 <= idx < |b[i].servers|;
+    assert 0 <= idx < |b[i+1].servers|;
+    assert b[i+1].servers[idx] != b[i].servers[idx];
+    var ios := lemma_ActionThatChangesServerIsThatServersAction(b, i, idx);
+    assert CMNextServer(b[i], b[i+1], idx, ios);
+    assert LServerNext(b[i].servers[idx], b[i+1].servers[idx], ios);
+    assert ServerValid(s);
+
+    assert ios[0].LIoOpReceive?;
+    var p := ios[0].r;
+    var sp := ExtractSentPacketsFromIos(ios);
+    assert p.msg.Message_Read? || p.msg.Message_Write? || p.msg.Message_Propagation?;
+
+    assert ServerProcessPacket(s, s', ios);
+
+    if p.msg.Message_Read? {
+        assert ReceiveRead(s, s', p, sp);
+        var (new_icache, new_ccache) := PullDeps2(s.icache, s.ccache, p.msg.deps_read);
+        lemma_PullDeps2DoneNotDecreaseVersions(s.icache, s.ccache, p.msg.deps_read);
+        assert s'.icache == new_icache;
+        assert s'.ccache == new_ccache;
+        assert CCacheDoesNotDecrease(s.ccache, s'.ccache);
+        assert ICacheDoesNotDecrease(s.icache, s'.icache);
+    } 
+    else if p.msg.Message_Write?
+    {
+        assert ReceiveWrite(s, s', p, sp);
+        assert CCacheDoesNotDecrease(s.ccache, s'.ccache);
+        assert ICacheDoesNotDecrease(s.icache, s'.icache);
+    }
+    else {
+        assert p.msg.Message_Propagation?;
+        assert ReceivePropagate(s, s', p, sp);
+        if s.next == p.msg.start {
+            var (new_icache, new_ccache) := PullDeps2(s.icache, s.ccache, p.msg.meta.deps);
+            lemma_PullDeps2DoneNotDecreaseVersions(s.icache, s.ccache, p.msg.meta.deps);
+            assert s'.icache == new_icache;
+            assert CCacheDoesNotDecrease(s.ccache, new_ccache);
+            var merged_meta := MetaMerge(new_ccache[p.msg.key], p.msg.meta);
+            var new_ccache' := InsertIntoCCache(new_ccache, merged_meta);
+            assert CCacheDoesNotDecrease(new_ccache, new_ccache');
+            // assert VCHappendsBefore(new_ccache[p.msg.key].vc, )
+            // assert s'.ccache == new_ccache;
+            assert CCacheDoesNotDecrease(s.ccache, s'.ccache);
+            assert ICacheDoesNotDecrease(s.icache, s'.icache);
+        }
+    }
+    assert CCacheDoesNotDecrease(s.ccache, s'.ccache);
+    assert ICacheDoesNotDecrease(s.icache, s'.icache);
+    assert forall j :: 0 <= j < |b[i].servers| && j != idx ==> 
+            b[i].servers[j].s.ccache == b[i+1].servers[j].s.ccache && b[i].servers[j].s.icache == b[i+1].servers[j].s.icache;
+    assert forall j :: 0 <= j < |b[i].servers| && j != idx ==>
+            CCacheDoesNotDecrease(b[i].servers[j].s.ccache, b[i+1].servers[j].s.ccache) 
+            && ICacheDoesNotDecrease(b[i].servers[j].s.icache, b[i+1].servers[j].s.icache);
+    lemma_CMNextCacheDoesNotDecrease_helper2(b, i, idx);
+    assert ServerNextDoesNotDecreaseVersions(b[i], b[i+1]);
+}
+
+lemma lemma_CMNextCacheDoesNotDecrease_helper2(b:Behavior<CMState>, i:int, idx:int)
+    requires IsValidBehaviorPrefix(b, i)
+    requires 0 <= i
+    requires 0 <= idx < |b[i].servers|
+    requires 0 <= idx < |b[i+1].servers|
+    requires b[i].servers[idx] != b[i+1].servers[idx]
+    // requires forall j :: 0 <= j < i ==> CMNext(b[j], b[j+1])
+    requires CMNext(b[i], b[i+1])
+    requires forall j :: 0 <= j < |b[i].servers| && j != idx ==>
+            CCacheDoesNotDecrease(b[i].servers[j].s.ccache, b[i+1].servers[j].s.ccache) 
+            && ICacheDoesNotDecrease(b[i].servers[j].s.icache, b[i+1].servers[j].s.icache)
+    requires CCacheDoesNotDecrease(b[i].servers[idx].s.ccache, b[i+1].servers[idx].s.ccache)
+    requires ICacheDoesNotDecrease(b[i].servers[idx].s.icache, b[i+1].servers[idx].s.icache)
+    ensures ServerNextDoesNotDecreaseVersions(b[i], b[i+1])
+{
+
+}
+
+lemma lemma_PullDeps2DoneNotDecreaseVersions(
+    icache:ICache, ccache:CCache, deps:Dependency
+)
+    requires ICacheValid(icache)
+    requires CCacheValid(ccache)
+    requires CausalCut(ccache)
+    requires forall k :: k in Keys_domain ==> k in icache && k in ccache
+    requires forall k :: k in ccache ==> k in icache
+    requires DependencyValid(deps)
+    requires forall k :: k in deps ==> k in icache
+    ensures var (new_icache, new_ccache) := PullDeps2(icache, ccache, deps);
+        CCacheDoesNotDecrease(ccache, new_ccache) && ICacheDoesNotDecrease(icache, new_icache)
+{
+    var domain := icache.Keys + deps.Keys;
+    var todos := GetMetasOfAllDeps(icache, deps, map[], domain);
+    var new_cache := MergeCCache(ccache, todos);
+    assert CCacheDoesNotDecrease(ccache, new_cache);
+
+    var (new_icache, new_ccache) := PullDeps2(icache, ccache, deps);
+    assert ICacheDoesNotDecrease(icache, new_icache);
+
+    assert new_ccache == new_cache;
+}
+
+}
