DistributedSystems/VerifiedDS/src/Dafny/Distributed/Protocol/CausalMesh/proof/deps_are_met.dfy
@@ -171,49 +171,51 @@ lemma lemma_MergeCCacheEnsuresAllVersionAreMetOnAllServers(
 //     // assert forall k :: k in merged ==> AVersionIsMetOnAllServers(b, i, k, merged[k].vc) && AllVersionsInDepsAreMetOnAllServers(b, i, merged[k].deps);
 // }
 
-lemma lemma_VersionsAfterPullDepsAreMetOnAllServers(
-    b:Behavior<CMState>,
-    i:int,
-    idx:int,
-    deps:Dependency
-)
-    requires i > 0
-    requires IsValidBehaviorPrefix(b, i)
-    requires CMNext(b[i-1], b[i])
-    requires 0 <= idx < Nodes
-    requires DependencyValid(deps)
-    requires AllDepsInICacheAreMetOnAllServers(b, i, b[i].servers[idx].s.icache)
-    requires AllVersionsInDepsAreMetOnAllServers(b, i, deps)
-    requires AllVersionsInCCacheAreMetOnAllServers(b, i, b[i].servers[idx].s.ccache)
-    ensures var res := PullDeps2(b[i].servers[idx].s.icache, b[i].servers[idx].s.ccache, deps);
-            AllVersionsInCCacheAreMetOnAllServers(b, i, res.1)
-{
-    reveal_AllVersionsInDepsAreMetOnAllServers();
-    reveal_AllDepsInICacheAreMetOnAllServers();
-    reveal_AllVersionsInCCacheAreMetOnAllServers();
-    assert CMNextCommon(b[i-1], b[i]);
-    var icache := b[i].servers[idx].s.icache;
-    var ccache := b[i].servers[idx].s.ccache;
-    var domain := icache.Keys + deps.Keys;
+// lemma lemma_VersionsAfterPullDepsAreMetOnAllServers(
+//     b:Behavior<CMState>,
+//     i:int,
+//     idx:int,
+//     deps:Dependency
+// )
+//     requires i > 0
+//     requires IsValidBehaviorPrefix(b, i)
+//     requires CMNext(b[i], b[i+1])
+//     requires 0 <= idx < Nodes
+//     requires DependencyValid(deps)
+//     requires AllDepsInICacheAreMetOnAllServers(b, i, b[i].servers[idx].s.icache)
+//     requires AllVersionsInDepsAreMetOnAllServers(b, i, deps)
+//     requires AllVersionsInCCacheAreMetOnAllServers(b, i, b[i].servers[idx].s.ccache)
+//     ensures var res := PullDeps2(b[i].servers[idx].s.icache, b[i].servers[idx].s.ccache, deps);
+//             AllVersionsInCCacheAreMetOnAllServers(b, i, res.1)
+// {
+//     lemma_BehaviorValidImpliesOneStepValid(b, i);
+//     reveal_AllVersionsInDepsAreMetOnAllServers();
+//     reveal_AllDepsInICacheAreMetOnAllServers();
+//     reveal_AllVersionsInCCacheAreMetOnAllServers();
+    
+//     // assert CMNextCommon(b[i-1], b[i]);
+//     var icache := b[i].servers[idx].s.icache;
+//     var ccache := b[i].servers[idx].s.ccache;
+//     var domain := icache.Keys + deps.Keys;
 
-    var todos := GetMetasOfAllDeps(icache, deps, map[], domain);
-    var todos1 := GetMetasOfAllDepsGlobalView(b, i, idx, icache, deps, map[], domain);
-    assert forall k :: k in todos1 ==> AVersionIsMetOnAllServers(b, i, k, todos1[k].vc) && AllVersionsInDepsAreMetOnAllServers(b, i, todos1[k].deps);
-    lemma_GetMetasOfAllDepsGlobalViewEqualsToGetMetasOfAllDeps(b, i, idx, icache, deps, map[], domain);
-    assert todos == todos1;
-    assert forall k :: k in todos ==> AVersionIsMetOnAllServers(b, i, k, todos[k].vc) && AllVersionsInDepsAreMetOnAllServers(b, i, todos[k].deps);
+//     var todos := GetMetasOfAllDeps(icache, deps, map[], domain);
+//     var todos1 := GetMetasOfAllDepsGlobalView(b, i, idx, icache, deps, map[], domain);
+//     assert forall k :: k in todos1 ==> AVersionIsMetOnAllServers(b, i, k, todos1[k].vc) && AllVersionsInDepsAreMetOnAllServers(b, i, todos1[k].deps);
+//     lemma_GetMetasOfAllDepsGlobalViewEqualsToGetMetasOfAllDeps(b, i, idx, icache, deps, map[], domain);
+//     assert todos == todos1;
+//     assert forall k :: k in todos ==> AVersionIsMetOnAllServers(b, i, k, todos[k].vc) && AllVersionsInDepsAreMetOnAllServers(b, i, todos[k].deps);
 
-    var new_cache := MergeCCache(ccache, todos);
-    lemma_MergeCCacheEnsuresAllVersionAreMetOnAllServers(b, i, ccache, todos);
-    assert AllVersionsInCCacheAreMetOnAllServers(b, i, new_cache);
+//     var new_cache := MergeCCache(ccache, todos);
+//     lemma_MergeCCacheEnsuresAllVersionAreMetOnAllServers(b, i, ccache, todos);
+//     assert AllVersionsInCCacheAreMetOnAllServers(b, i, new_cache);
 
-    var res := PullDeps2(icache, ccache, deps);
-    assert res.1 == new_cache;
-    assert AllVersionsInCCacheAreMetOnAllServers(b, i, res.1);
-    // assert AllVersionsInCCacheAreMetOnAllServers(b, i, new_cache);
-    // assume AllVersionsInDepsAreMetOnAllServers(b, i, deps);
-    // assume AllVersionsInCCacheAreMetOnAllServers(b, i, ccache);
-}
+//     var res := PullDeps2(icache, ccache, deps);
+//     assert res.1 == new_cache;
+//     assert AllVersionsInCCacheAreMetOnAllServers(b, i, res.1);
+//     // assert AllVersionsInCCacheAreMetOnAllServers(b, i, new_cache);
+//     // assume AllVersionsInDepsAreMetOnAllServers(b, i, deps);
+//     // assume AllVersionsInCCacheAreMetOnAllServers(b, i, ccache);
+// }
 
 lemma {:axiom} lemma_AllMeatsAreMetImpliesMergedMetaIsMet(
     b:Behavior<CMState>,
@@ -255,121 +257,206 @@ lemma {:axiom} lemma_MetaMapIsMetImpliesInsertedMataMapIsMet(
 
 // }
 
+// function GetMetasOfAllDepsGlobalView(
+//     b:Behavior<CMState>,
+//     i:int,
+//     idx:int,
+//     icache:ICache,
+//     deps:Dependency,
+//     todos:map<Key, Meta>,
+//     domain:set<Key>
+// ) : (res:map<Key, Meta>)
+//     requires i > 0
+//     requires IsValidBehaviorPrefix(b, i)
+//     requires CMNext(b[i-1], b[i])
+//     requires forall k :: k in icache ==> k in Keys_domain && (forall m :: m in icache[k] ==> MetaValid(m) && m.key == k
+//                 && (forall kk :: kk in m.deps ==> kk in domain && kk in Keys_domain))
+//     requires DependencyValid(deps)
+//     requires forall k :: k in todos ==> MetaValid(todos[k]) && todos[k].key == k 
+//     requires forall k :: k in Keys_domain ==> k in icache // should we have this?
+//     requires forall k :: k in deps ==> k in domain 
 
-function GetMetasOfAllDepsGlobalView(
-    b:Behavior<CMState>,
-    i:int,
-    idx:int,
-    icache:ICache,
-    deps:Dependency,
-    todos:map<Key, Meta>,
-    domain:set<Key>
-) : (res:map<Key, Meta>)
-    requires i > 0
-    requires IsValidBehaviorPrefix(b, i)
-    requires CMNext(b[i-1], b[i]);
-    requires forall k :: k in icache ==> k in Keys_domain && (forall m :: m in icache[k] ==> MetaValid(m) && m.key == k
-                && (forall kk :: kk in m.deps ==> kk in domain && kk in Keys_domain))
-    requires DependencyValid(deps)
-    requires forall k :: k in todos ==> MetaValid(todos[k]) && todos[k].key == k 
-    requires forall k :: k in Keys_domain ==> k in icache // should we have this?
-    requires forall k :: k in deps ==> k in domain 
+//     requires AllDepsInICacheAreMetOnAllServers(b, i, icache)
+//     requires AllVersionsInDepsAreMetOnAllServers(b, i, deps)
+//     requires forall k :: k in todos ==> AVersionIsMetOnAllServers(b, i, k, todos[k].vc) && AllVersionsInDepsAreMetOnAllServers(b, i, todos[k].deps)
 
-    requires AllDepsInICacheAreMetOnAllServers(b, i, icache)
-    requires AllVersionsInDepsAreMetOnAllServers(b, i, deps)
-    requires forall k :: k in todos ==> AVersionIsMetOnAllServers(b, i, k, todos[k].vc) && AllVersionsInDepsAreMetOnAllServers(b, i, todos[k].deps)
-
-    ensures forall k :: k in res ==> MetaValid(res[k]) && res[k].key == k 
-    ensures forall k :: k in res ==> AVersionIsMetOnAllServers(b, i, k, res[k].vc) && AllVersionsInDepsAreMetOnAllServers(b, i, res[k].deps)
-    decreases |icache.Values|, |deps|
-{
-    reveal_AllVersionsInDepsAreMetOnAllServers();
-    reveal_AllDepsInICacheAreMetOnAllServers();
-    reveal_AllVersionsInCCacheAreMetOnAllServers();
-    assert forall k :: k in todos ==> AVersionIsMetOnAllServers(b, i, k, todos[k].vc) && AllVersionsInDepsAreMetOnAllServers(b, i, todos[k].deps);
-    if |deps| == 0 then 
-        todos
-    else 
-        var k :| k in deps;
-        var new_deps := RemoveElt(deps, k);
-        if k in todos && (VCHappendsBefore(deps[k], todos[k].vc) || VCEq(deps[k], todos[k].vc)) then 
-            var res := GetMetasOfAllDepsGlobalView(b, i, idx, icache, new_deps, todos, domain);
-            res
-        else 
-            var metas := set m | m in icache[k] && (VCHappendsBefore(m.vc, deps[k]) || VCEq(m.vc, deps[k]));
-            if |metas| > 0 then 
-                var initial := EmptyMeta(k);
-                var merged := FoldMetaSet(initial, metas, domain);
-                var meta := merged.(vc := deps[k]);
+//     ensures forall k :: k in res ==> MetaValid(res[k]) && res[k].key == k 
+//     ensures forall k :: k in res ==> AVersionIsMetOnAllServers(b, i, k, res[k].vc) && AllVersionsInDepsAreMetOnAllServers(b, i, res[k].deps)
+//     decreases |icache.Values|, |deps|
+// {
+//     // lemma_BehaviorValidImpliesOneStepValid(b, i);
+//     reveal_AllVersionsInDepsAreMetOnAllServers();
+//     reveal_AllDepsInICacheAreMetOnAllServers();
+//     reveal_AllVersionsInCCacheAreMetOnAllServers();
+    
+//     assert forall k :: k in todos ==> AVersionIsMetOnAllServers(b, i, k, todos[k].vc) && AllVersionsInDepsAreMetOnAllServers(b, i, todos[k].deps);
+//     if |deps| == 0 then 
+//         todos
+//     else 
+//         var k :| k in deps;
+//         var new_deps := RemoveElt(deps, k);
+//         if k in todos && (VCHappendsBefore(deps[k], todos[k].vc) || VCEq(deps[k], todos[k].vc)) then 
+//             var res := GetMetasOfAllDepsGlobalView(b, i, idx, icache, new_deps, todos, domain);
+//             res
+//         else 
+//             var metas := set m | m in icache[k] && (VCHappendsBefore(m.vc, deps[k]) || VCEq(m.vc, deps[k]));
+//             if |metas| > 0 then 
+//                 var initial := EmptyMeta(k);
+//                 var merged := FoldMetaSet(initial, metas, domain);
+//                 var meta := merged.(vc := deps[k]);
                 
                 
-                lemma_FoldMetaBounded(initial, metas, deps[k], domain);
-                assert (VCHappendsBefore(merged.vc, meta.vc) || VCEq(merged.vc, meta.vc));
+//                 lemma_FoldMetaBounded(initial, metas, deps[k], domain);
+//                 assert (VCHappendsBefore(merged.vc, meta.vc) || VCEq(merged.vc, meta.vc));
 
-                var new_cache := icache[k:= icache[k] - metas];
-                assert icache[k] >= metas;
-                lemma_MapRemoveSubsetOfTheValOfKey(icache, k, metas);
-                assert |new_cache.Values| < |icache.Values|;
+//                 var new_cache := icache[k:= icache[k] - metas];
+//                 assert icache[k] >= metas;
+//                 lemma_MapRemoveSubsetOfTheValOfKey(icache, k, metas);
+//                 assert |new_cache.Values| < |icache.Values|;
 
-                assert AllDepsInICacheAreMetOnAllServers(b, i, new_cache);
-                lemma_AllMeatsAreMetImpliesMergedMetaIsMet(b, i, initial, metas, domain);
-                assert AllVersionsInDepsAreMetOnAllServers(b, i, merged.deps);
+//                 assert AllDepsInICacheAreMetOnAllServers(b, i, new_cache);
+//                 lemma_AllMeatsAreMetImpliesMergedMetaIsMet(b, i, initial, metas, domain);
+//                 assert AllVersionsInDepsAreMetOnAllServers(b, i, merged.deps);
 
-                var res := GetMetasOfAllDepsGlobalView(b, i, idx, new_cache, merged.deps, todos, domain);
+//                 var res := GetMetasOfAllDepsGlobalView(b, i, idx, new_cache, merged.deps, todos, domain);
 
-                assert forall k :: k in res ==> AVersionIsMetOnAllServers(b, i, k, res[k].vc) && AllVersionsInDepsAreMetOnAllServers(b, i, res[k].deps);
-                assert AVersionIsMetOnAllServers(b, i, k, meta.vc);
+//                 assert forall k :: k in res ==> AVersionIsMetOnAllServers(b, i, k, res[k].vc) && AllVersionsInDepsAreMetOnAllServers(b, i, res[k].deps);
+//                 assert AVersionIsMetOnAllServers(b, i, k, meta.vc);
 
-                var todos' := AddMetaToMetaMap(res, meta);
+//                 var todos' := AddMetaToMetaMap(res, meta);
 
-                assert AllVersionsInDepsAreMetOnAllServers(b, i, new_deps);
-                lemma_MetaMapIsMetImpliesInsertedMataMapIsMet(b, i, res, meta);
-                assert forall k :: k in todos' ==> AVersionIsMetOnAllServers(b, i, k, todos'[k].vc) && AllVersionsInDepsAreMetOnAllServers(b, i, todos'[k].deps);
+//                 assert AllVersionsInDepsAreMetOnAllServers(b, i, new_deps);
+//                 lemma_MetaMapIsMetImpliesInsertedMataMapIsMet(b, i, res, meta);
+//                 assert forall k :: k in todos' ==> AVersionIsMetOnAllServers(b, i, k, todos'[k].vc) && AllVersionsInDepsAreMetOnAllServers(b, i, todos'[k].deps);
 
-                var res' := GetMetasOfAllDepsGlobalView(b, i, idx, icache, new_deps, todos', domain);
-                res'
-            else 
-                var initial := EmptyMeta(k);
-                var meta := initial.(vc:=deps[k]);
+//                 var res' := GetMetasOfAllDepsGlobalView(b, i, idx, icache, new_deps, todos', domain);
+//                 res'
+//             else 
+//                 var initial := EmptyMeta(k);
+//                 var meta := initial.(vc:=deps[k]);
                 
-                var todos' := AddMetaToMetaMap(todos, meta);
+//                 var todos' := AddMetaToMetaMap(todos, meta);
                 
-                var res := GetMetasOfAllDepsGlobalView(b, i, idx, icache, new_deps, todos', domain);
-                res
-}
+//                 var res := GetMetasOfAllDepsGlobalView(b, i, idx, icache, new_deps, todos', domain);
+//                 res
+// }
+
+// function GetMetasOfAllDepsGlobalView(
+//     b:Behavior<CMState>,
+//     i:int,
+//     idx:int,
+//     icache:ICache,
+//     deps:Dependency,
+//     todos:map<Key, Meta>,
+//     domain:set<Key>
+// ) : (res:map<Key, Meta>)
+//     requires i > 0
+//     requires IsValidBehaviorPrefix(b, i)
+//     requires CMNext(b[i-1], b[i])
+//     requires forall k :: k in icache ==> k in Keys_domain && (forall m :: m in icache[k] ==> MetaValid(m) && m.key == k
+//                 && (forall kk :: kk in m.deps ==> kk in domain && kk in Keys_domain))
+//     requires DependencyValid(deps)
+//     requires forall k :: k in todos ==> MetaValid(todos[k]) && todos[k].key == k 
+//     requires forall k :: k in Keys_domain ==> k in icache // should we have this?
+//     requires forall k :: k in deps ==> k in domain 
+
+//     requires AllDepsInICacheAreMetOnAllServers(b, i, icache)
+//     requires AllVersionsInDepsAreMetOnAllServers(b, i, deps)
+//     requires forall k :: k in todos ==> AVersionIsMetOnAllServers(b, i, k, todos[k].vc) && AllVersionsInDepsAreMetOnAllServers(b, i, todos[k].deps)
+
+//     ensures forall k :: k in res ==> MetaValid(res[k]) && res[k].key == k 
+//     ensures forall k :: k in res ==> AVersionIsMetOnAllServers(b, i, k, res[k].vc) && AllVersionsInDepsAreMetOnAllServers(b, i, res[k].deps)
+//     decreases |icache.Values|, |deps|
+// {
+//     // lemma_BehaviorValidImpliesOneStepValid(b, i);
+//     reveal_AllVersionsInDepsAreMetOnAllServers();
+//     reveal_AllDepsInICacheAreMetOnAllServers();
+//     reveal_AllVersionsInCCacheAreMetOnAllServers();
+    
+//     assert forall k :: k in todos ==> AVersionIsMetOnAllServers(b, i, k, todos[k].vc) && AllVersionsInDepsAreMetOnAllServers(b, i, todos[k].deps);
+//     if |deps| == 0 then 
+//         todos
+//     else 
+//         var k :| k in deps;
+//         var new_deps := RemoveElt(deps, k);
+//         if k in todos && (VCHappendsBefore(deps[k], todos[k].vc) || VCEq(deps[k], todos[k].vc)) then 
+//             var res := GetMetasOfAllDepsGlobalView(b, i, idx, icache, new_deps, todos, domain);
+//             res
+//         else 
+//             var metas := set m | m in icache[k] && (VCHappendsBefore(m.vc, deps[k]) || VCEq(m.vc, deps[k]));
+//             if |metas| > 0 then 
+//                 var initial := EmptyMeta(k);
+//                 var merged := FoldMetaSet(initial, metas, domain);
+//                 var meta := merged.(vc := deps[k]);
+                
+                
+//                 lemma_FoldMetaBounded(initial, metas, deps[k], domain);
+//                 assert (VCHappendsBefore(merged.vc, meta.vc) || VCEq(merged.vc, meta.vc));
+
+//                 var new_cache := icache[k:= icache[k] - metas];
+//                 assert icache[k] >= metas;
+//                 lemma_MapRemoveSubsetOfTheValOfKey(icache, k, metas);
+//                 assert |new_cache.Values| < |icache.Values|;
+
+//                 assert AllDepsInICacheAreMetOnAllServers(b, i, new_cache);
+//                 lemma_AllMeatsAreMetImpliesMergedMetaIsMet(b, i, initial, metas, domain);
+//                 assert AllVersionsInDepsAreMetOnAllServers(b, i, merged.deps);
+
+//                 var res := GetMetasOfAllDepsGlobalView(b, i, idx, new_cache, merged.deps, todos, domain);
+
+//                 assert forall k :: k in res ==> AVersionIsMetOnAllServers(b, i, k, res[k].vc) && AllVersionsInDepsAreMetOnAllServers(b, i, res[k].deps);
+//                 assert AVersionIsMetOnAllServers(b, i, k, meta.vc);
+
+//                 var todos' := AddMetaToMetaMap(res, meta);
+
+//                 assert AllVersionsInDepsAreMetOnAllServers(b, i, new_deps);
+//                 lemma_MetaMapIsMetImpliesInsertedMataMapIsMet(b, i, res, meta);
+//                 assert forall k :: k in todos' ==> AVersionIsMetOnAllServers(b, i, k, todos'[k].vc) && AllVersionsInDepsAreMetOnAllServers(b, i, todos'[k].deps);
+
+//                 var res' := GetMetasOfAllDepsGlobalView(b, i, idx, icache, new_deps, todos', domain);
+//                 res'
+//             else 
+//                 var initial := EmptyMeta(k);
+//                 var meta := initial.(vc:=deps[k]);
+                
+//                 var todos' := AddMetaToMetaMap(todos, meta);
+                
+//                 var res := GetMetasOfAllDepsGlobalView(b, i, idx, icache, new_deps, todos', domain);
+//                 res
+// }
 
 // lemma {:axiom} lemma_TwoMetaMapAreEqual(m1:map<Key, Meta>, m2:map<Key, Meta>)
 //     ensures m1 == m2
 
-lemma {:axiom} lemma_GetMetasOfAllDepsGlobalViewEqualsToGetMetasOfAllDeps
-(
-    b:Behavior<CMState>,
-    i:int,
-    idx:int,
-    icache:ICache,
-    deps:Dependency,
-    todos:map<Key, Meta>,
-    domain:set<Key>
-)
-    requires i > 0
-    requires IsValidBehaviorPrefix(b, i)
-    requires CMNext(b[i-1], b[i]);
-    requires forall k :: k in icache ==> k in Keys_domain && (forall m :: m in icache[k] ==> MetaValid(m) && m.key == k
-                && (forall kk :: kk in m.deps ==> kk in domain && kk in Keys_domain))
-    requires DependencyValid(deps)
-    requires forall k :: k in todos ==> MetaValid(todos[k]) && todos[k].key == k 
-    requires forall k :: k in Keys_domain ==> k in icache // should we have this?
-    requires forall k :: k in deps ==> k in domain 
+// lemma {:axiom} lemma_GetMetasOfAllDepsGlobalViewEqualsToGetMetasOfAllDeps
+// (
+//     b:Behavior<CMState>,
+//     i:int,
+//     idx:int,
+//     icache:ICache,
+//     deps:Dependency,
+//     todos:map<Key, Meta>,
+//     domain:set<Key>
+// )
+//     requires i > 0
+//     requires IsValidBehaviorPrefix(b, i)
+//     requires CMNext(b[i-1], b[i]);
+//     requires forall k :: k in icache ==> k in Keys_domain && (forall m :: m in icache[k] ==> MetaValid(m) && m.key == k
+//                 && (forall kk :: kk in m.deps ==> kk in domain && kk in Keys_domain))
+//     requires DependencyValid(deps)
+//     requires forall k :: k in todos ==> MetaValid(todos[k]) && todos[k].key == k 
+//     requires forall k :: k in Keys_domain ==> k in icache // should we have this?
+//     requires forall k :: k in deps ==> k in domain 
 
-    requires forall k :: k in todos ==> forall kk :: kk in todos[k].deps ==> 
-                        VCHappendsBefore(todos[k].deps[kk], todos[k].vc) || VCEq(todos[k].deps[kk], todos[k].vc)
-    requires CausalCut(todos)
+//     requires forall k :: k in todos ==> forall kk :: kk in todos[k].deps ==> 
+//                         VCHappendsBefore(todos[k].deps[kk], todos[k].vc) || VCEq(todos[k].deps[kk], todos[k].vc)
+//     requires CausalCut(todos)
 
-    requires AllDepsInICacheAreMetOnAllServers(b, i, icache)
-    requires AllVersionsInDepsAreMetOnAllServers(b, i, deps)
-    requires forall k :: k in todos ==> AVersionIsMetOnAllServers(b, i, k, todos[k].vc) && AllVersionsInDepsAreMetOnAllServers(b, i, todos[k].deps)
-    ensures 
-            var res1 := GetMetasOfAllDepsGlobalView(b, i, idx, icache, deps, todos, domain);
-            var res2 := GetMetasOfAllDeps(icache, deps, todos, domain);
-            res1 == res2
+//     requires AllDepsInICacheAreMetOnAllServers(b, i, icache)
+//     requires AllVersionsInDepsAreMetOnAllServers(b, i, deps)
+//     requires forall k :: k in todos ==> AVersionIsMetOnAllServers(b, i, k, todos[k].vc) && AllVersionsInDepsAreMetOnAllServers(b, i, todos[k].deps)
+//     ensures 
+//             var res1 := GetMetasOfAllDepsGlobalView(b, i, idx, icache, deps, todos, domain);
+//             var res2 := GetMetasOfAllDeps(icache, deps, todos, domain);
+//             res1 == res2
 }
