DistributedSystems/VerifiedDS/src/Dafny/Distributed/Protocol/CausalMesh/proof/servers_are_met.dfy
@@ -1,0 +1,155 @@
+include "../distributed_system.dfy"
+include "packet_sending.dfy"
+include "properties.dfy"
+include "environment.dfy"
+include "deps_are_met.dfy"
+include "read_reply_is_met.dfy"
+include "../../../Common/Collections/Seqs.s.dfy"
+
+module CausalMesh_Proof_ServersAreMet_i {
+import opened CausalMesh_Cache_i
+import opened CausalMesh_Message_i
+import opened CausalMesh_Types_i
+import opened Environment_s
+import opened CausalMesh_DistributedSystem_i
+import opened CausalMesh_Properties_i
+import opened CausalMesh_PullDeps_i
+import opened CausalMesh_Proof_Actions_i
+import opened Temporal__Temporal_s
+import opened CausalMesh_proof_Assumptions_i
+import opened CausalMesh_Proof_Constants_i
+import opened CausalMesh_Proof_PacketSending_i
+import opened CausalMesh_Proof_Properties_i
+import opened CausalMesh_Proof_Environment_i
+import opened CausalMesh_Proof_DepsAreMet_i
+import opened CausalMesh_Proof_ReadReplyIsMet_i
+import opened Collections__Seqs_s
+import opened Collections__Maps_i
+import opened Collections__Maps2_s
+
+lemma lemma_ServersAreMetForCMNext(b:Behavior<CMState>, i:int, idx:int)
+    requires IsValidBehaviorPrefix(b, i+1)
+    requires 0 < i
+    requires 0 <= idx < |b[i].servers|
+    requires 0 <= idx < |b[i+1].servers|
+    requires b[i].servers[idx] != b[i+1].servers[idx]
+    requires CMNext(b[i], b[i+1])
+    requires AllServersAreMet(b, i)
+    requires AllVersionsInCCacheAreMetOnAllServers(b, i, b[i].servers[idx].s.ccache)
+    // requires AllVersionsInDepsAreMetOnAllServers(b, i-1, p.msg.deps_read)
+    requires AllDepsInICacheAreMetOnAllServers(b, i, b[i].servers[idx].s.icache)
+    requires AllReadDepsAreMet(b, i)
+    requires ServerNextDoesNotDecreaseVersions(b[i], b[i+1])
+    // ensures AllServersAreMet(b, i+1)
+{
+    var s := b[i].servers[idx].s;
+    var s' := b[i+1].servers[idx].s;
+
+    var ios := lemma_ActionThatChangesServerIsThatServersAction(b, i, idx);
+    assert CMNextServer(b[i], b[i+1], idx, ios);
+    assert LServerNext(b[i].servers[idx], b[i+1].servers[idx], ios);
+    assert ServerValid(s);
+
+    assert ios[0].LIoOpReceive?;
+    var p := ios[0].r;
+    var sp := ExtractSentPacketsFromIos(ios);
+    assert p.msg.Message_Read? || p.msg.Message_Write? || p.msg.Message_Propagation?;
+    assert p in b[i].environment.sentPackets;
+
+    // lemma_BehaviorValidImpliesOneStepValid(b, i-1);
+
+    assert ServerProcessPacket(s, s', ios);
+    if p.msg.Message_Read? {
+        assert ReceiveRead(s, s', p, sp);
+        var (new_icache, new_ccache) := PullDeps2(s.icache, s.ccache, p.msg.deps_read);
+        assert AllReadDepsAreMet(b, i);
+        assert forall pp :: pp in b[i].environment.sentPackets && pp.msg.Message_Read? ==> 
+            AllVersionsInDepsAreMetOnAllServers(b, i, pp.msg.deps_read);
+        assert AllVersionsInDepsAreMetOnAllServers(b, i, p.msg.deps_read);
+        lemma_VersionsAfterPullDepsAreMetOnAllServers(b, i, idx, p.msg.deps_read);
+        
+        assert AllVersionsInCCacheAreMetOnAllServers(b, i, new_ccache);
+
+        lemma_CCacheIsMetOnAllServersWillAlwaysMet(b, i+1, new_ccache);
+        lemma_ICacheIsMetOnAllServersWillAlwaysMet(b, i+1, new_icache);
+        assert s'.icache == new_icache;
+        assert s'.ccache == new_ccache;
+        assert AllVersionsInCCacheAreMetOnAllServers(b, i+1, b[i+1].servers[idx].s.ccache);
+        assert AllDepsInICacheAreMetOnAllServers(b, i+1, b[i+1].servers[idx].s.icache);
+    } 
+    else if p.msg.Message_Write?
+    {
+        assert ReceiveWrite(s, s', p, sp);
+        assert s'.icache == s.icache;
+        assert s'.ccache == s.ccache;
+        lemma_CCacheIsMetOnAllServersWillAlwaysMet(b, i+1, s.ccache);
+        assert AllVersionsInCCacheAreMetOnAllServers(b, i+1, b[i+1].servers[idx].s.ccache);
+    }
+}
+
+
+lemma lemma_CCacheIsMetOnAllServersWillAlwaysMet(
+    b:Behavior<CMState>,
+    i:int,
+    ccache:CCache
+)
+    requires 1 < i
+    requires IsValidBehaviorPrefix(b, i)
+    requires CMNext(b[i-1], b[i])
+    requires CCacheValid(ccache)
+    requires ServerNextDoesNotDecreaseVersions(b[i-1], b[i])
+    requires AllVersionsInCCacheAreMetOnAllServers(b, i-1, ccache)
+    ensures AllVersionsInCCacheAreMetOnAllServers(b, i, ccache)
+{
+    assert i-1 > 0;
+    assert IsValidBehaviorPrefix(b, i-1);
+    lemma_BehaviorValidImpliesOneStepValid(b, i-1);
+    reveal_AllVersionsInCCacheAreMetOnAllServers();
+
+    forall k | k in ccache
+        ensures AVersionIsMetOnAllServers(b, i, k, ccache[k].vc)
+        ensures AllVersionsInDepsAreMetOnAllServers(b, i, ccache[k].deps)
+    {
+        assert AVersionIsMetOnAllServers(b, i-1, k, ccache[k].vc);
+        lemma_AVersionIsMetOnAllServersWillAlwaysMet(b, i, k, ccache[k].vc);
+        lemma_AllVersionsInDepsAreMetOnAllServersWillAlwaysMet(b, i, ccache[k].deps);
+    }
+}
+
+lemma lemma_ICacheIsMetOnAllServersWillAlwaysMet(
+    b:Behavior<CMState>,
+    i:int,
+    icache:ICache
+)
+    requires 1 < i
+    requires IsValidBehaviorPrefix(b, i)
+    requires CMNext(b[i-1], b[i])
+    requires ICacheValid(icache)
+    requires ServerNextDoesNotDecreaseVersions(b[i-1], b[i])
+    requires AllDepsInICacheAreMetOnAllServers(b, i-1, icache)
+    ensures AllDepsInICacheAreMetOnAllServers(b, i, icache)
+{
+    assert i-1 > 0;
+    assert IsValidBehaviorPrefix(b, i-1);
+    lemma_BehaviorValidImpliesOneStepValid(b, i-1);
+    reveal_AllDepsInICacheAreMetOnAllServers();
+
+    forall k | k in icache
+    {
+        forall m:Meta | m in icache[k] 
+        {
+            forall kk | kk in m.deps 
+                ensures AVersionIsMetOnAllServers(b, i, kk, m.deps[kk])
+            {
+                assert AVersionIsMetOnAllServers(b, i-1, kk, m.deps[kk]);
+                lemma_AVersionIsMetOnAllServersWillAlwaysMet(b, i, kk, m.deps[kk]);
+                assert AVersionIsMetOnAllServers(b, i, kk, m.deps[kk]);
+            }
+        }
+    }
+
+    assert forall k :: k in icache ==>
+            forall m:Meta :: m in icache[k] ==> 
+                forall kk :: kk in m.deps ==> AVersionIsMetOnAllServers(b, i, kk, m.deps[kk]);
+}
+}
